template-coq/theories/ExtractLoopChecking.v
@@ -1,6 +1,6 @@
 From Equations Require Import Equations.
 From Coq Require Import ExtrOcamlBasic ExtrOcamlNatInt ExtrOcamlZInt.
-From MetaCoq.Template Require Import clauses.
+From MetaCoq.Template Require Import LoopChecking.
 
 Extract Constant BinInt.Z.of_nat => "(fun x -> x)".
 Extract Constant BinInt.Z.to_nat => "(fun x -> x)".
@@ -8,13 +8,10 @@ Extract Constant pr1 => "fst".
 Extract Constant pr2 => "snd".
 
 Extraction Inline inspect.
-Extraction Inline levelexpr_level levelexpr_value premise concl.
-Extraction Inline model_model.
-Extraction Inline infer_result.
 Extraction Inline ReflectEq.eqb ReflectEq.reflect_prod ReflectEq.eq_prod.
 
 Cd "extraction_clauses".
 
-Extraction "clauses.ml" infer infer_extension enforce_cstrs.
+Extraction "loop_checking.ml" LoopChecking.
 
 Cd "..".
